llvm/codeflow/element.ml
@@ -7,8 +7,7 @@ module MakeStatement (E:Exp) = struct
   module Exp = E
   type t =
     | Comment of string
-    | Assign of (Exp.code * Exp.t option * Exp.t list)
-    | Load of (Exp.t * Exp.t)
+    | Assign of (bool * Exp.code * Exp.t option * Exp.t list)
     | MutInd of (string * Exp.t * t) list
     | Loop of (Exp.t list * t)
     | Bind of (Exp.t list * t * t)
@@ -16,8 +15,7 @@ module MakeStatement (E:Exp) = struct
     | Dangling (* non'a tinate statement *)
     | Raise of int
 
-  let mkAssign c lhs ops = Assign (c, lhs, ops)
-  let mkLoad v ptr = Load (v, ptr)
+  let mkAssign b c lhs ops = Assign (b, c, lhs, ops)
   let mkMutInd cases = MutInd cases
   let mkLoop ctx ts = Loop (ctx, ts)
   let mkFallThrough _ = FallThrough
@@ -39,23 +37,51 @@ module MakeStatement (E:Exp) = struct
      | Bind (x, s1, s2) -> Bind (x, s1, bind v s2 app)
      | _ -> Bind (v, arg, app)
 
-  let rec emit_ctx emitter ctx s = match s with
+  let rec collect_context ctx s =
+    match s with
+    | Bind (v, _, _) -> v @ ctx
+    | MutInd ((_,_,s) :: tl)-> begin
+        List.fold_left (fun ctx (_,_,s) ->
+          collect_context ctx s
+        ) (collect_context ctx s) tl
+      end
+    | _ -> ctx
+
+  let add_context ctx v =
+    let add_one ctx c =
+      try
+        let _ = List.iter (fun e ->
+          if e == c then raise (Failure "Found") else ()
+        ) ctx in
+        raise Not_found
+      with
+        | Failure _ -> ctx
+        | Not_found -> c :: ctx
+    in
+    List.fold_left (fun acc v -> add_one acc v) ctx v
+
+  let rec emit_ctx emitter ctx s =
+    match s with
     | Comment s -> Emitter.emitLine emitter "(* %s *)" s; ctx
     | Bind (v, s1, s2) -> begin
-        let ctx = v @ ctx in
+        let ctx = add_context ctx v in
         let ctx = emit_ctx emitter ctx s1 in
         emit_ctx emitter ctx s2
       end
     | MutInd ls -> begin
+        Emitter.emitLine emitter "(* context: %s *)" (string_of_ctx ctx);
+        let ctx = collect_context ctx s in
         let _, cond, _ = List.hd ls in
-        Emitter.emitLine emitter "let _ = match %s with" (Exp.to_string cond);
-        let emitter = Emitter.indent emitter in
+        Emitter.emitLine emitter "__context %%= match %s with"
+          (*string_of_ctx ctx*) (Exp.to_string cond);
+        let emitter' = Emitter.indent emitter in
         ignore @@ List.map (fun (e,_,s) ->
-          Emitter.emitLine emitter "%s =>" e;
-          let emitter' = Emitter.indent emitter in
+          Emitter.emitLine emitter' "| %s =>" e;
+          let emitter' = Emitter.indent emitter' in
           emit_ctx emitter' ctx s
         ) ls;
-        Emitter.emitLine emitter "in";
+        Emitter.emitLine emitter "end;";
+        Emitter.emitLine emitter "let %s = __context in" (string_of_ctx ctx);
         ctx
       end
     | Loop (lctx, s) -> begin
@@ -67,23 +93,19 @@ module MakeStatement (E:Exp) = struct
       end
     | Raise c -> Emitter.emitLine emitter "raise %d" c; ctx
     | FallThrough -> begin
-        Emitter.emitLine emitter "%s" (string_of_ctx ctx);
+        Emitter.emitLine emitter "ret %s" (string_of_ctx ctx);
         Emitter.emitLine emitter "(* fallthrough *)";
         ctx
       end
     | Dangling -> Emitter.emitLine emitter "dangling"; ctx
-    | Load (x, y) -> begin
-        Emitter.emitLine emitter "%s <- load %s;"
-          (Exp.to_string x) (Exp.to_string y);
-        ctx
-      end
-    | Assign (op, lhs, ops) -> begin
+    | Assign (pure, op, lhs, ops) -> begin
         let rhs = List.fold_left (fun acc operand ->
               acc ^ " " ^  (Exp.to_string operand)
           ) (Exp.code_to_string op) ops in
         let _ = match lhs with
-          | Some lhs -> Emitter.emitLine emitter "%s ?= %s;"
-              (Exp.to_string lhs) rhs
+          | Some lhs -> Emitter.emitLine emitter "%s %%= %s;"
+              (Exp.to_string lhs)
+              (if pure then "ret (" ^ rhs ^ ")" else rhs)
           | None -> Emitter.emitLine emitter "%s;;" rhs
         in ctx
       end
