llvm/codeflow/element.mli
@@ -4,8 +4,7 @@ module MakeStatement:
   functor (E:Exp) -> sig
   module Exp : (Exp with type t = E.t and type code = E.code)
   type t
-  val mkAssign: Exp.code -> Exp.t option -> Exp.t list -> t
-  val mkLoad: Exp.t -> Exp.t -> t
+  val mkAssign: bool -> Exp.code -> Exp.t option -> Exp.t list -> t
   val mkMutInd: (string * Exp.t * t) list -> t
   val mkLoop: Exp.t list -> t -> t
   val mkFallThrough: unit -> t
