llvm/funcBuilder.ml
@@ -1,16 +1,35 @@
 open Lltrans.Utils
 
 let phi_lattice = Hashtbl.create 20
-
-module LlvmValue = struct
-  type t = Llvm.llvalue
-  type code = Llvm.Opcode.t
-  let code_to_string = op_to_string
-  let to_string a = value_to_string a
-end
+let phi_table = Hashtbl.create 20
 
 let emit_llfun_body emitter llfun =
+  let repr_table = Hashtbl.create 20 in
+  let temp_counter = ref 0 in
+
+  let add_repr lli =
+    match Llvm.classify_value lli with
+    | Llvm.ValueKind.Instruction _ -> begin
+        let name = Llvm.value_name lli in
+        let name = if name = "" then begin
+          temp_counter := !temp_counter + 1;
+          "___ssa" ^ (string_of_int !temp_counter)
+        end else
+          List.hd (String.split_on_char '.' name)
+        in Hashtbl.replace repr_table lli name
+      end
+    | _ -> ()
+  in
+
+  let module LlvmValue = struct
+    type t = Llvm.llvalue
+    type code = (* Llvm.Opcode.t *) string
+    let code_to_string c = c
+    let to_string a = value_to_string (fun c -> Hashtbl.find repr_table c) a
+  end in
+
   let module ValueMap = Map.Make(String) in
+
   let bbmap, _ = Llvm.fold_left_blocks (fun (map,i) llb ->
     let llv = Llvm.value_of_block llb in
     let llname = Llvm.value_name llv in
@@ -19,11 +38,18 @@ let emit_llfun_body emitter llfun =
 
   let _ = Llvm.fold_left_blocks (fun _ bb->
     Llvm.fold_left_instrs (fun () v ->
-       update_phi_lattice (fun _ src lli ->
-         if (is_phi_value src) then begin
-           Hashtbl.add phi_lattice src lli
-         end else ()
-       ) v
+      add_repr v;
+      update_phi_lattice (fun b src lli ->
+        if (is_phi_value src) then begin
+          Hashtbl.add phi_lattice src lli
+        end else if (is_constant src) then begin
+          let phi_claims = match Hashtbl.find_opt phi_table b with
+            | None -> Hashtbl.add phi_table b []; []
+            | Some ls -> ls
+          in
+          Hashtbl.replace phi_table b ((lli,src) :: phi_claims)
+        end else ()
+      ) v
     ) () bb
   ) () llfun in
 
@@ -35,7 +61,7 @@ let emit_llfun_body emitter llfun =
     | _ -> lli
   in
 
-  let module Translator = Lltrans.FuncBuilder.Translator (LlvmValue) in
+  let module Translator = Lltrans.BlockBuilder.Translator (LlvmValue) in
   let module BB = BasicBlock (struct
     let get_block_id na = ValueMap.find na bbmap
   end) (Translator.LlvmStatement.Exp) in
@@ -50,16 +76,16 @@ let emit_llfun_body emitter llfun =
   let aggregate = CFG.aggregate entry_block bset false in
   let st = CFG.trace aggregate (CFG.Statement.mkFallThrough ())
     aggregate None (Llvm.value_of_block entry_block, entry_block)
-    (Translator.translator var_lattice)
+    (Translator.translator var_lattice phi_table)
   in
   CFG.Statement.emit emitter (snd st)
 
 let emit_llfun llfun =
-  if (Lltrans.FuncBuilder.is_debug_fun_decl llfun) then
+  if (Lltrans.BlockBuilder.is_debug_fun_decl llfun) then
     ()
   else begin
     let emitter = Codeflow.Emitter.indent @@ Codeflow.Emitter.mkEmitter () in
-    Lltrans.FuncBuilder.emit_func_head llfun;
+    Lltrans.BlockBuilder.emit_func_head llfun;
     emit_llfun_body emitter llfun;
     Printf.printf "\n";
     ()
