llvm/lltrans/blockBuilder.mli
@@ -9,8 +9,12 @@ val is_debug_fun_decl: Llvm.llvalue -> bool
 module Translator:
   functor (LlvmValue: Exp.Exp with
     type t = Llvm.llvalue and
-    type code = Llvm.Opcode.t
+    type code = string
   ) -> sig
   module LlvmStatement: Cfg.Statement with module Exp = LlvmValue
-  val translator: llvalue_lattice -> Llvm.llbasicblock -> (Llvm.llvalue * LlvmStatement.t) * ((string * Llvm.llvalue * Llvm.llbasicblock) list)
+  val translator:
+        llvalue_lattice
+     -> (Llvm.llbasicblock, (Llvm.llvalue * Llvm.llvalue) list) Hashtbl.t
+     -> Llvm.llbasicblock
+     -> (Llvm.llvalue * LlvmStatement.t) * ((string * Llvm.llvalue * Llvm.llbasicblock) list)
 end
