llvm/specBuilder.ml
@@ -1,21 +1,33 @@
-let _ =
+open Core
+let do_compile src_file =
   let llctx = Llvm.global_context () in
-  let llmem = Llvm.MemoryBuffer.of_file Sys.argv.(1) in
+  let llmem = Llvm.MemoryBuffer.of_file src_file in
   let llm = Llvm_bitreader.parse_bitcode llctx llmem in
 
-  Llvm.dump_module llm;
-  (* Uncomment this for debugging purpose
+  (*
+   * Uncomment this for debugging purpose
    * Llvm.dump_module llm;
    *)
 
   Llvm.iter_functions FuncBuilder.emit_llfun llm;
 
   let emitter = Codeflow.Emitter.mkEmitter () in
-  Lltrans.TypeBuilder.emit_types emitter;
+  ignore @@ Lltrans.TypeBuilder.emit_types emitter
 
   (*
-  Printf.printf "*** iter_globals ***\n";
-  Llvm.iter_globals print_val llm;
-  *)
+   * Printf.printf "*** iter_globals ***\n";
+   * Llvm.iter_globals print_val llm;
+   *)
 
-  ()
+let command =
+  Command.basic
+    ~summary:"Translate .bc files into a coq specification"
+    ~readme:(fun () -> "More detailed information")
+    Command.Param.(
+     map (anon ("filename" %: string))
+       ~f:(fun filename -> (fun () -> do_compile filename)))
+
+let () =
+  Command.run ~version:"1.0" ~build_info:"RWO" command
+
+
