theories/wprules.v
@@ -16,11 +16,14 @@ Qed.
 
 Lemma
   get_obj_wp
-  {Forward: Type}
-  {type_ind: type_of_ind Forward}
-  ft ref Q :
-  { fun s => Q (dereference ref ft s) s }
-    [| get_obj ref ft |]
+  {type_ind: Type}
+  {ind: type_ind}
+  {otype:Type}
+  {ti: type_of_ind ind otype}
+  (ref:reference ind)
+  Q :
+  { fun s => Q (dereference ref s) s }
+    [| get_obj ref |]
   { Q }.
 Proof.
   unfold hoare_triple, bind, get_obj in *.
@@ -29,11 +32,13 @@ Qed.
 
 Lemma
   set_obj_wp
-  {Forward: Type}
-  {type_ind: type_of_ind Forward}
-  {ft: Forward}
-  (o: (@to Forward) type_ind ft)
-  ref Q :
+  {type_ind: Type}
+  {ind: type_ind}
+  {otype: Type}
+  {ti: type_of_ind ind otype}
+  (o: otype)
+  (ref: reference ind)
+  Q :
   { fun s => Q tt (set_memory s (set ref o)) }
     [| set_obj o ref |]
   { Q }.
